Monoid_TheoryよりMonoidStructureの方が分かりやすかろう

monoid.v
@@ -1,23 +1,23 @@
 (* coq8.3 *)
 (* normalization by evalutionとproof by reflectionの練習 *)
 
-Section Monoid_Theory_def.
-  Variable M : Type.
-  Variable Mop : M -> M -> M.
-  Variable Mid : M.
+Record MonoidStructure (M:Type) := {
+  Mop : M -> M -> M;
+  Mid : M;
+  Mop_assoc : forall a b c:M , Mop a (Mop b c) = Mop (Mop a b) c;
+  Mop_lunit : forall a:M , Mop Mid a = a;
+  Mop_runit : forall a:M , Mop a Mid = a }.
 
-  Record Monoid_Theory : Prop := 
-  { Mop_assoc : forall a b c:M , Mop a (Mop b c) = Mop (Mop a b) c;
-    Mop_lunit : forall a:M , Mop Mid a = a;
-    Mop_runit : forall a:M , Mop a Mid = a }.
-End Monoid_Theory_def.
+Implicit Arguments Mop [M].
+Implicit Arguments Mid [M].
+Implicit Arguments Mop_assoc [M].
+Implicit Arguments Mop_runit [M].
+Implicit Arguments Mop_lunit [M].
 
 
-Section Monoid_reflect.
-  Variable M : Type.
-  Variable Mop : M -> M -> M.
-  Variable Mid : M.
-  Variable T : Monoid_Theory M Mop Mid.
+Section MonoidReflect.
+  Variable M:Type.
+  Variable T:MonoidStructure M.
 
   Inductive MonoidTerm :=
     | identity : MonoidTerm
@@ -32,29 +32,30 @@ Section Monoid_reflect.
        exact (fun x => (M1 (M2 x))).
   Defined.
 
-  Definition normalize : MonoidTerm -> MonoidTerm := (fun x => embed x identity).
+  Definition normalize : MonoidTerm -> MonoidTerm := 
+     (fun x => embed x identity).
 
   Definition eval : MonoidTerm -> M.
-    intro x;induction x as [ | a | _ M1 _ M2].
-       exact Mid.
-       exact a.
-       exact (Mop M1 M2).
+     intro x;induction x as [ | a | _ M1 _ M2].
+        exact (Mid T).
+        exact a.
+        exact (Mop T M1 M2).
   Defined.
 
   Lemma op_eq_embed : forall (e e':MonoidTerm),eval (op e e') = eval (embed e e').
      intro e;induction e as [ | a | e1 M1 e2 M2].
         idtac "case of identity".
-           exact (fun x => Mop_lunit _ _ _  T (eval x)).
+           exact (fun x => Mop_lunit T (eval x)).
         idtac "case of var a".
            reflexivity.
         idtac "case of var e1 e2".
-           assert(H:forall x y,eval (op x y)=Mop (eval x) (eval y)) by reflexivity.
+           assert(H:forall x y,eval (op x y)=Mop T (eval x) (eval y)) by reflexivity.
            intro e';simpl.
            rewrite <- (M1 (embed e2 e')).
            rewrite (H e1 (embed e2 e')).
            rewrite <- (M2 e').
            rewrite (H e2 e').
-           apply eq_sym;exact (Mop_assoc _ _ _ T _ _ _).
+           apply eq_sym;exact (Mop_assoc T _ _ _).
   Qed.
 
   Theorem monoid_reflect : forall (e e':MonoidTerm),normalize e=normalize e' -> eval e=eval e'.
@@ -62,8 +63,8 @@ Section Monoid_reflect.
      assert(P:forall t,eval (normalize t) = eval t).
        intro t.
        assert(P1:=op_eq_embed t identity).
-       assert(P2:=Mop_runit _ _ _ T (eval t)).
-       assert(P3:eval (op t identity)=Mop (eval t) Mid) by reflexivity.
+       assert(P2:=Mop_runit T (eval t)).
+       assert(P3:eval (op t identity)=Mop T (eval t) (Mid T)) by reflexivity.
        unfold normalize;congruence.
      assert(H1 : eval (normalize e) = eval e) by (exact (P e)).
      assert(H2 : eval (normalize e') = eval e') by (exact (P e')).
@@ -71,29 +72,25 @@ Section Monoid_reflect.
   Qed.
 
   (*
-    -- 逆はいえない
-    -- eval nat plus 0 (op (var 1) (var 2)) = eval nat plus 0 (var 3)
-    -- but , normalize nat (op (var 1) (var 2)) <> normalize nat (var 3).
+-- 逆はいえない
+-- @eval nat nat_is_monoid (op (var 1) (var 2)) = @eval nat nat_is_monoid (var 3)
+-- but , normalize nat (op (var 1) (var 2)) <> normalize nat (var 3).
    *)
-End Monoid_reflect.
+End MonoidReflect.
 
 Implicit Arguments var [M].
 Implicit Arguments op [M].
-Implicit Arguments monoid_reflect [M Mop Mid].
+Implicit Arguments monoid_reflect [M].
+Implicit Arguments eval [M].
 
-
-(* 例 *)
 Require Import List.
 Goal forall X (x y z w :list X),(x++y)++(z++w)=((x++y)++z)++w.
    intros X x y z w.
    set (e1:=op (op (var x) (var y)) (op (var z) (var w))).
    set (e2:=op (op (op (var x) (var y)) (var z)) (var w)).
-   assert(Lmth : Monoid_Theory (list X) (@app X) nil).
-      apply Build_Monoid_Theory.
-      apply app_assoc.
-      apply app_nil_l.
-      apply app_nil_r.
+   set (Lmth := Build_MonoidStructure _ _ _ (@app_assoc X) (@app_nil_l X) (@app_nil_r X)).
    apply (monoid_reflect Lmth e1 e2);compute;reflexivity.
 Qed.
+
 
 
